Jan21-Isab/compare.thy
@@ -1,0 +1,40 @@
+theory compare
+  imports Main "/Volumes/Setup/Isabelle/Isabelle-Code/Jan21-Isab/trinhlibs"
+begin
+(*BIP*)
+value "\<exists>bet \<in> set t_betaSet_1. (
+  \<forall>j \<in> set t_SyncInstance_1. \<forall>u \<in> set j. \<exists>t \<in> set u.\<exists>l \<in> set (snd t).(
+    (\<not>P (fst t) l 
+    \<and> (\<forall>elm \<in> set bet.\<forall>el1 \<in> set elm.\<forall>h \<in> set (lookup_3 (fst el1) t_TrigInstance_1) - {snd el1}. \<not>Q (fst el1) h) 
+    \<and> (\<forall>l1 \<in> set (snd t) - {l}. \<not> P (fst t) l1))
+\<or> 
+  (\<forall>elm \<in> set bet.\<exists>el1 \<in> set elm. Q (fst el1) (snd el1) 
+\<and> (\<forall>elm \<in> set bet.\<forall>el1 \<in> set elm.\<forall>h \<in> set (lookup_3 (fst el1) t_TrigInstance_1) - {snd el1}. \<not>Q (fst el1) h) 
+\<and> (\<forall>l1 \<in> set (snd t) - {l}. \<not> P (fst t) l1)))
+)"
+
+(*JavaBIP*)
+value "((\<forall>j \<in> set t_SyncInstance_1. \<forall>u \<in> set j.\<forall>t \<in> set u. \<forall>l \<in> set (snd t). \<not>P (fst t) l) 
+\<and> (\<forall>i \<in> set t_TrigInstance_1. \<forall>v \<in> set i. \<forall>k \<in> set v. \<exists>h \<in> set (snd k).\<forall>h1 \<in> set (snd k) - {h}. \<not> Q (fst k) h1))
+\<or> ((\<exists>bet \<in> set t_betaSet_1. (\<forall>elm \<in> set bet.\<exists>el1 \<in> set elm. Q (fst el1) (snd el1)) 
+\<and> (\<forall>elm \<in> set bet.\<forall>el1 \<in> set elm.\<forall>h \<in> set (lookup_3 (fst el1) t_TrigInstance_1) - {snd el1}. \<not>Q (fst el1) h)) 
+\<and> (\<forall>j \<in> set t_SyncInstance_1. \<forall>u \<in> set j. \<forall>t \<in> set u. \<exists>l \<in> set (snd t).\<forall>l1 \<in> set (snd t) - {l}. \<not> P (fst t)  l1))"
+
+lemma compare1:
+"\<exists>bet \<in> set t_betaSet_1. (
+  \<forall>j \<in> set t_SyncInstance_1. \<forall>u \<in> set j. \<exists>t \<in> set u.\<exists>l \<in> set (snd t).(
+    (\<not>P (fst t) l 
+    \<and> (\<forall>elm \<in> set bet.\<forall>el1 \<in> set elm.\<forall>h \<in> set (lookup_3 (fst el1) t_TrigInstance_1) - {snd el1}. \<not>Q (fst el1) h) 
+    \<and> (\<forall>l1 \<in> set (snd t) - {l}. \<not> P (fst t) l1))
+\<or> 
+  (\<forall>elm \<in> set bet.\<exists>el1 \<in> set elm. Q (fst el1) (snd el1) 
+\<and> (\<forall>elm \<in> set bet.\<forall>el1 \<in> set elm.\<forall>h \<in> set (lookup_3 (fst el1) t_TrigInstance_1) - {snd el1}. \<not>Q (fst el1) h) 
+\<and> (\<forall>l1 \<in> set (snd t) - {l}. \<not> P (fst t) l1)))
+)
+\<Longrightarrow> ((\<forall>j \<in> set t_SyncInstance_1. \<forall>u \<in> set j.\<forall>t \<in> set u. \<forall>l \<in> set (snd t). \<not>P (fst t) l) 
+\<and> (\<forall>i \<in> set t_TrigInstance_1. \<forall>v \<in> set i. \<forall>k \<in> set v. \<exists>h \<in> set (snd k).\<forall>h1 \<in> set (snd k) - {h}. \<not> Q (fst k) h1))
+\<or> ((\<exists>bet \<in> set t_betaSet_1. (\<forall>elm \<in> set bet.\<exists>el1 \<in> set elm. Q (fst el1) (snd el1)) 
+\<and> (\<forall>elm \<in> set bet.\<forall>el1 \<in> set elm.\<forall>h \<in> set (lookup_3 (fst el1) t_TrigInstance_1) - {snd el1}. \<not>Q (fst el1) h)) 
+\<and> (\<forall>j \<in> set t_SyncInstance_1. \<forall>u \<in> set j. \<forall>t \<in> set u. \<exists>l \<in> set (snd t).\<forall>l1 \<in> set (snd t) - {l}. \<not> P (fst t)  l1))"
+
+end
