Jan21-Isab/javabip.thy
@@ -6,18 +6,25 @@ value "t_betaSet_1"
 value "mk_pair_4 t_TrigInstance_1"
 
 (*---- JavaBIP encoding ----*)
+(*
+(\<not>P(t,l) \<or> (Q(el1, el1) \<and> \<not>Q(el1,h))) \<and> \<not>P(t,l1) \<and> \<not>Q(k,h1)
+\<equiv> [\<not>P(t,l) \<and> \<not>P(t,l1) \<and> \<not>Q(k,h1)] \<or> [Q(el1, el1) \<and> \<not>Q(el1,h) \<and> \<not>P(t,l1) \<and> \<not>Q(k,h1)]
+*)
 value "(\<forall>j \<in> set t_SyncInstance_1. \<forall>u \<in> set j.\<forall>t \<in> set u. \<forall>l \<in> set (snd t). \<not>P (fst t) l \<or> (\<exists>bet \<in> set t_betaSet_1. (\<forall>elm \<in> set bet.\<exists>el1 \<in> set elm. Q (fst el1) (snd el1)) \<and> (\<forall>elm \<in> set bet.\<forall>el1 \<in> set elm.\<forall>h \<in> set (lookup_3 (fst el1) t_TrigInstance_1) - {snd el1}. \<not>Q (fst el1) h)))
 \<and> (\<forall>j \<in> set t_SyncInstance_1. \<forall>u \<in> set j. \<forall>t \<in> set u. \<exists>l \<in> set (snd t).\<forall>l1 \<in> set (snd t) - {l}. \<not> P (fst t) l1) 
 \<and> (\<forall>i \<in> set t_TrigInstance_1. \<forall>v \<in> set i. \<forall>k \<in> set v. \<exists>h \<in> set (snd k).\<forall>h1 \<in> set (snd k) - {h}. \<not> Q (fst k) h1)"
 
 (*---- JavaBIP encoding - 1st transform ----*)
+(*[\<not>P(t,l) \<and> \<not>P(t,l1) \<and> \<not>Q(k,h1)]*)
 value "((\<forall>j \<in> set t_SyncInstance_1. \<forall>u \<in> set j.\<forall>t \<in> set u. \<forall>l \<in> set (snd t). \<not>P (fst t) l) 
 \<and> (\<forall>j \<in> set t_SyncInstance_1. \<forall>u \<in> set j. \<forall>t \<in> set u. \<exists>l \<in> set (snd t).\<forall>l1 \<in> set (snd t) - {l}. \<not> P (fst t)  l1) 
 \<and> (\<forall>i \<in> set t_TrigInstance_1. \<forall>v \<in> set i. \<forall>k \<in> set v. \<exists>h \<in> set (snd k).\<forall>h1 \<in> set (snd k) - {h}. \<not> Q (fst k) h1))" 
 
+(*[Q(el1, el1) \<and> \<not>Q(el1,h) \<and> \<not>P(t,l1) \<and> \<not>Q(k,h1)]*)
 value "((\<exists>bet \<in> set t_betaSet_1. (\<forall>elm \<in> set bet.\<exists>el1 \<in> set elm. Q (fst el1) (snd el1)) \<and> (\<forall>elm \<in> set bet.\<forall>el1 \<in> set elm.\<forall>h \<in> set (lookup_3 (fst el1) t_TrigInstance_1) - {snd el1}. \<not>Q (fst el1) h)) \<and> (\<forall>j \<in> set t_SyncInstance_1. \<forall>u \<in> set j. \<forall>t \<in> set u. \<exists>l \<in> set (snd t).\<forall>l1 \<in> set (snd t) - {l}. \<not> P (fst t)  l1) 
 \<and> (\<forall>i \<in> set t_TrigInstance_1. \<forall>v \<in> set i. \<forall>k \<in> set v. \<exists>h \<in> set (snd k).\<forall>h1 \<in> set (snd k) - {h}. \<not> Q (fst k) h1))" 
 
+(*[\<not>P(t,l) \<and> \<not>P(t,l1) \<and> \<not>Q(k,h1)] \<or> [Q(el1, el1) \<and> \<not>Q(el1,h) \<and> \<not>P(t,l1) \<and> \<not>Q(k,h1)]*)
 value "
 ((\<forall>j \<in> set t_SyncInstance_1. \<forall>u \<in> set j.\<forall>t \<in> set u. \<forall>l \<in> set (snd t). \<not>P (fst t) l) 
 \<and> (\<forall>j \<in> set t_SyncInstance_1. \<forall>u \<in> set j. \<forall>t \<in> set u. \<exists>l \<in> set (snd t).\<forall>l1 \<in> set (snd t) - {l}. \<not> P (fst t)  l1) 
@@ -41,10 +48,9 @@ lemma fst_transform: "(\<forall>j \<in> set t_SyncInstance_1. \<forall>u \<in> s
   by blast
 
 (*---- JavaBIP encoding - 2nd transform ----*)
-value "((\<forall>j \<in> set t_SyncInstance_1. \<forall>u \<in> set j.\<forall>t \<in> set u. \<forall>l \<in> set (snd t). \<not>P (fst t) l) 
+(*[Q(el1, el1) \<and> \<not>Q(el1,h) \<and> \<not>P(t,l1) \<and> \<not>Q(k,h1)]*)
+value "((\<exists>bet \<in> set t_betaSet_1. (\<forall>elm \<in> set bet.\<exists>el1 \<in> set elm. Q (fst el1) (snd el1)) \<and> (\<forall>elm \<in> set bet.\<forall>el1 \<in> set elm.\<forall>h \<in> set (lookup_3 (fst el1) t_TrigInstance_1) - {snd el1}. \<not>Q (fst el1) h)) \<and> (\<forall>j \<in> set t_SyncInstance_1. \<forall>u \<in> set j. \<forall>t \<in> set u. \<exists>l \<in> set (snd t).\<forall>l1 \<in> set (snd t) - {l}. \<not> P (fst t)  l1)
 \<and> (\<forall>i \<in> set t_TrigInstance_1. \<forall>v \<in> set i. \<forall>k \<in> set v. \<exists>h \<in> set (snd k).\<forall>h1 \<in> set (snd k) - {h}. \<not> Q (fst k) h1))" 
-
-value "((\<exists>bet \<in> set t_betaSet_1. (\<forall>elm \<in> set bet.\<exists>el1 \<in> set elm. Q (fst el1) (snd el1)) \<and> (\<forall>elm \<in> set bet.\<forall>el1 \<in> set elm.\<forall>h \<in> set (lookup_3 (fst el1) t_TrigInstance_1) - {snd el1}. \<not>Q (fst el1) h)) \<and> (\<forall>j \<in> set t_SyncInstance_1. \<forall>u \<in> set j. \<forall>t \<in> set u. \<exists>l \<in> set (snd t).\<forall>l1 \<in> set (snd t) - {l}. \<not> P (fst t)  l1))" 
 
 value "((\<forall>j \<in> set t_SyncInstance_1. \<forall>u \<in> set j.\<forall>t \<in> set u. \<forall>l \<in> set (snd t). \<not>P (fst t) l) 
 \<and> (\<forall>i \<in> set t_TrigInstance_1. \<forall>v \<in> set i. \<forall>k \<in> set v. \<exists>h \<in> set (snd k).\<forall>h1 \<in> set (snd k) - {h}. \<not> Q (fst k) h1))
@@ -68,4 +74,8 @@ lemma snd_transform: "
 
 value "((\<forall>j \<in> set t_SyncInstance_1. \<forall>u \<in> set j.\<forall>t \<in> set u. \<forall>l \<in> set (snd t). \<not>P (fst t) l) 
 \<and> (\<forall>i \<in> set t_TrigInstance_1. \<forall>v \<in> set i. \<forall>k \<in> set v. \<exists>h \<in> set (snd k).\<forall>h1 \<in> set (snd k) - {h}. \<not> Q (fst k) h1))"
+
+value "((\<forall>j \<in> set t_SyncInstance_1. \<forall>u \<in> set j.\<forall>t \<in> set u. \<forall>l \<in> set (snd t). \<not>P (fst t) l) 
+\<and> (\<forall>i \<in> set t_TrigInstance_1. \<forall>v \<in> set i. \<forall>k \<in> set v. \<exists>h \<in> set (snd k).\<forall>h1 \<in> set (snd k) - {h}. \<not> Q (fst k) h1))
+\<or> ((\<exists>bet \<in> set t_betaSet_1. (\<forall>elm \<in> set bet.\<exists>el1 \<in> set elm. Q (fst el1) (snd el1)) \<and> (\<forall>elm \<in> set bet.\<forall>el1 \<in> set elm.\<forall>h \<in> set (lookup_3 (fst el1) t_TrigInstance_1) - {snd el1}. \<not>Q (fst el1) h)) \<and> (\<forall>j \<in> set t_SyncInstance_1. \<forall>u \<in> set j. \<forall>t \<in> set u. \<exists>l \<in> set (snd t).\<forall>l1 \<in> set (snd t) - {l}. \<not> P (fst t)  l1))"
 end
