Jan21-Isab/javabip_1.thy
@@ -1,0 +1,57 @@
+theory javabip_1
+  imports Main "/Volumes/Setup/Isabelle/Isabelle-Code/Jan21-Isab/trinhlibs"
+begin
+(*---- JavaBIP encoding ----*)
+(*
+(\<not>P(t,l) \<or> (Q(el1, el1) \<and> \<not>Q(el1,h))) \<and> \<not>P(t,l1) \<and> \<not>Q(k,h1)
+\<equiv> [\<not>P(t,l) \<and> \<not>P(t,l1) \<and> \<not>Q(k,h1)] \<or> [Q(el1, el1) \<and> \<not>Q(el1,h) \<and> \<not>P(t,l1) \<and> \<not>Q(k,h1)]
+*)
+value "(\<forall>j \<in> set t_SyncInstance_1. \<forall>u \<in> set j.\<forall>t \<in> set u. \<forall>l \<in> set (snd t). \<not>P (fst t) l \<or> (\<exists>bet \<in> set t_betaSet_1. (\<forall>elm \<in> set bet.\<exists>el1 \<in> set elm. Q (fst el1) (snd el1)) \<and> (\<forall>elm \<in> set bet.\<forall>el1 \<in> set elm.\<forall>h \<in> set (lookup_3 (fst el1) t_TrigInstance_1) - {snd el1}. \<not>Q (fst el1) h)))
+\<and> (\<forall>j \<in> set t_SyncInstance_1. \<forall>u \<in> set j. \<forall>t \<in> set u. \<exists>l \<in> set (snd t).\<forall>l1 \<in> set (snd t) - {l}. \<not> P (fst t) l1) 
+\<and> (\<forall>i \<in> set t_TrigInstance_1. \<forall>v \<in> set i. \<forall>k \<in> set v. \<exists>h \<in> set (snd k).\<forall>h1 \<in> set (snd k) - {h}. \<not> Q (fst k) h1)"
+
+(*[\<not>P(t,l) \<and> \<not>P(t,l1) \<and> \<not>Q(k,h1)]*)
+value "(\<forall>j \<in> set t_SyncInstance_1. \<forall>u \<in> set j.\<forall>t \<in> set u. \<forall>l \<in> set (snd t). \<not>P (fst t) l) 
+\<and> (\<forall>j \<in> set t_SyncInstance_1. \<forall>u \<in> set j. \<forall>t \<in> set u. \<exists>l \<in> set (snd t).\<forall>l1 \<in> set (snd t) - {l}. \<not> P (fst t)  l1) 
+\<and> (\<forall>i \<in> set t_TrigInstance_1. \<forall>v \<in> set i. \<forall>k \<in> set v. \<exists>h \<in> set (snd k).\<forall>h1 \<in> set (snd k) - {h}. \<not> Q (fst k) h1)"
+
+(*\<not>P(t,l) \<and> \<not>P(t,l1) \<and> \<not>Q(k,h1)
+\<equiv> \<not>P(t,l) \<and> \<not>Q(k,h1) *)
+lemma rutgon_1:"
+((\<forall>j \<in> set t_SyncInstance_1. \<forall>u \<in> set j.\<forall>t \<in> set u. \<forall>l \<in> set (snd t). \<not>P (fst t) l) 
+\<and> (\<forall>j \<in> set t_SyncInstance_1. \<forall>u \<in> set j. \<forall>t \<in> set u. \<exists>l \<in> set (snd t).\<forall>l1 \<in> set (snd t) - {l}. \<not> P (fst t)  l1)
+\<and> (\<forall>i \<in> set t_TrigInstance_1. \<forall>v \<in> set i. \<forall>k \<in> set v. \<exists>h \<in> set (snd k).\<forall>h1 \<in> set (snd k) - {h}. \<not> Q (fst k) h1))
+\<Longrightarrow> ((\<forall>j \<in> set t_SyncInstance_1. \<forall>u \<in> set j.\<forall>t \<in> set u. \<forall>l \<in> set (snd t). \<not>P (fst t) l)
+\<and> (\<forall>i \<in> set t_TrigInstance_1. \<forall>v \<in> set i. \<forall>k \<in> set v. \<exists>h \<in> set (snd k).\<forall>h1 \<in> set (snd k) - {h}. \<not> Q (fst k) h1))
+"
+  by simp
+
+(*[Q(el1, el1) \<and> \<not>Q(el1,h) \<and> \<not>P(t,l1) \<and> \<not>Q(k,h1)]*)
+value "((\<exists>bet \<in> set t_betaSet_1. (\<forall>elm \<in> set bet.\<exists>el1 \<in> set elm. Q (fst el1) (snd el1)) \<and> (\<forall>elm \<in> set bet.\<forall>el1 \<in> set elm.\<forall>h \<in> set (lookup_3 (fst el1) t_TrigInstance_1) - {snd el1}. \<not>Q (fst el1) h)) \<and> (\<forall>j \<in> set t_SyncInstance_1. \<forall>u \<in> set j. \<forall>t \<in> set u. \<exists>l \<in> set (snd t).\<forall>l1 \<in> set (snd t) - {l}. \<not> P (fst t)  l1)
+\<and> (\<forall>i \<in> set t_TrigInstance_1. \<forall>v \<in> set i. \<forall>k \<in> set v. \<exists>h \<in> set (snd k).\<forall>h1 \<in> set (snd k) - {h}. \<not> Q (fst k) h1))" 
+
+(*[Q(el1, el1) \<and> \<not>Q(el1,h) \<and> \<not>P(t,l1)]*)
+value "((\<exists>bet \<in> set t_betaSet_1. (\<forall>elm \<in> set bet.\<exists>el1 \<in> set elm. Q (fst el1) (snd el1)) \<and> (\<forall>elm \<in> set bet.\<forall>el1 \<in> set elm.\<forall>h \<in> set (lookup_3 (fst el1) t_TrigInstance_1) - {snd el1}. \<not>Q (fst el1) h)) \<and> (\<forall>j \<in> set t_SyncInstance_1. \<forall>u \<in> set j. \<forall>t \<in> set u. \<exists>l \<in> set (snd t).\<forall>l1 \<in> set (snd t) - {l}. \<not> P (fst t)  l1))" 
+
+(*[Q(el1, el1) \<and> \<not>Q(el1,h) \<and> \<not>P(t,l1) \<and> \<not>Q(k,h1)]
+\<equiv> [Q(el1, el1) \<and> \<not>Q(el1,h) \<and> \<not>P(t,l1)]
+*)
+lemma rutgon_2:"((\<exists>bet \<in> set t_betaSet_1. (\<forall>elm \<in> set bet.\<exists>el1 \<in> set elm. Q (fst el1) (snd el1)) \<and> (\<forall>elm \<in> set bet.\<forall>el1 \<in> set elm.\<forall>h \<in> set (lookup_3 (fst el1) t_TrigInstance_1) - {snd el1}. \<not>Q (fst el1) h)) \<and> (\<forall>j \<in> set t_SyncInstance_1. \<forall>u \<in> set j. \<forall>t \<in> set u. \<exists>l \<in> set (snd t).\<forall>l1 \<in> set (snd t) - {l}. \<not> P (fst t)  l1)
+\<and> (\<forall>i \<in> set t_TrigInstance_1. \<forall>v \<in> set i. \<forall>k \<in> set v. \<exists>h \<in> set (snd k).\<forall>h1 \<in> set (snd k) - {h}. \<not> Q (fst k) h1))
+\<Longrightarrow>((\<exists>bet \<in> set t_betaSet_1. (\<forall>elm \<in> set bet.\<exists>el1 \<in> set elm. Q (fst el1) (snd el1)) \<and> (\<forall>elm \<in> set bet.\<forall>el1 \<in> set elm.\<forall>h \<in> set (lookup_3 (fst el1) t_TrigInstance_1) - {snd el1}. \<not>Q (fst el1) h)) \<and> (\<forall>j \<in> set t_SyncInstance_1. \<forall>u \<in> set j. \<forall>t \<in> set u. \<exists>l \<in> set (snd t).\<forall>l1 \<in> set (snd t) - {l}. \<not> P (fst t)  l1)) "
+  by simp
+
+(*check after 2 shortened*)
+lemma sau2rg: "((\<forall>j \<in> set t_SyncInstance_1. \<forall>u \<in> set j.\<forall>t \<in> set u. \<forall>l \<in> set (snd t). \<not>P (fst t) l \<or> (\<exists>bet \<in> set t_betaSet_1. (\<forall>elm \<in> set bet.\<exists>el1 \<in> set elm. Q (fst el1) (snd el1)) \<and> (\<forall>elm \<in> set bet.\<forall>el1 \<in> set elm.\<forall>h \<in> set (lookup_3 (fst el1) t_TrigInstance_1) - {snd el1}. \<not>Q (fst el1) h)))
+\<and> (\<forall>j \<in> set t_SyncInstance_1. \<forall>u \<in> set j. \<forall>t \<in> set u. \<exists>l \<in> set (snd t).\<forall>l1 \<in> set (snd t) - {l}. \<not> P (fst t) l1) 
+\<and> (\<forall>i \<in> set t_TrigInstance_1. \<forall>v \<in> set i. \<forall>k \<in> set v. \<exists>h \<in> set (snd k).\<forall>h1 \<in> set (snd k) - {h}. \<not> Q (fst k) h1))
+\<Longrightarrow> ((\<forall>j \<in> set t_SyncInstance_1. \<forall>u \<in> set j.\<forall>t \<in> set u. \<forall>l \<in> set (snd t). \<not>P (fst t) l)
+\<and> (\<forall>i \<in> set t_TrigInstance_1. \<forall>v \<in> set i. \<forall>k \<in> set v. \<exists>h \<in> set (snd k).\<forall>h1 \<in> set (snd k) - {h}. \<not> Q (fst k) h1)
+\<or> (\<exists>bet \<in> set t_betaSet_1. (\<forall>elm \<in> set bet.\<exists>el1 \<in> set elm. Q (fst el1) (snd el1)) \<and> (\<forall>elm \<in> set bet.\<forall>el1 \<in> set elm.\<forall>h \<in> set (lookup_3 (fst el1) t_TrigInstance_1) - {snd el1}. \<not>Q (fst el1) h)) \<and> (\<forall>j \<in> set t_SyncInstance_1. \<forall>u \<in> set j. \<forall>t \<in> set u. \<exists>l \<in> set (snd t).\<forall>l1 \<in> set (snd t) - {l}. \<not> P (fst t)  l1))"
+  by blast
+
+(*JavaBIP \<equiv> [\<not>P(t,l) \<and> \<not>Q(k,h1)] \<or> [Q(el1, el1) \<and> \<not>Q(el1,h) \<and> \<not>P(t,l1)]*)
+value "((\<forall>j \<in> set t_SyncInstance_1. \<forall>u \<in> set j.\<forall>t \<in> set u. \<forall>l \<in> set (snd t). \<not>P (fst t) l)
+\<and> (\<forall>i \<in> set t_TrigInstance_1. \<forall>v \<in> set i. \<forall>k \<in> set v. \<exists>h \<in> set (snd k).\<forall>h1 \<in> set (snd k) - {h}. \<not> Q (fst k) h1)
+\<or> (\<exists>bet \<in> set t_betaSet_1. (\<forall>elm \<in> set bet.\<exists>el1 \<in> set elm. Q (fst el1) (snd el1)) \<and> (\<forall>elm \<in> set bet.\<forall>el1 \<in> set elm.\<forall>h \<in> set (lookup_3 (fst el1) t_TrigInstance_1) - {snd el1}. \<not>Q (fst el1) h)) \<and> (\<forall>j \<in> set t_SyncInstance_1. \<forall>u \<in> set j. \<forall>t \<in> set u. \<exists>l \<in> set (snd t).\<forall>l1 \<in> set (snd t) - {l}. \<not> P (fst t)  l1))"
+end
